examples/Imp2Vir/CFGC_Interface.v
@@ -1,0 +1,363 @@
+From Coq Require Import
+     Lists.List
+     Strings.String
+     FSets.FMapList
+     Structures.OrderedTypeEx
+     ZArith.
+Module Import StringMap := Coq.FSets.FMapList.Make(String_as_OT).
+
+From ExtLib Require Import
+     Structures.Monads
+     Data.Monads.OptionMonad.
+Import MonadNotation.
+
+From Vellvm Require Import
+     Syntax
+     SurfaceSyntax .
+
+From Imp2Vir Require Import Imp CFGC_Combinators CFGC_Utils.
+
+
+Import ListNotations.
+Import VIR_Notations.
+Notation ocfg := (ocfg typ).
+
+Record dcfg : Type :=
+  make_dcfg { graph : ocfg ;
+    ins : (list block_id * nat) ;
+    outs : (list block_id * nat) }.
+
+Definition mk_dcfg g (ins outs : list block_id)
+  : dcfg :=
+  {| graph := g;
+    ins := (ins, List.length ins) ;
+    outs := (outs, List.length outs) |}.
+
+Section FreshnessMonad.
+
+  Definition mk_anon (n : nat) := Anon (Z.of_nat n).
+  Definition name := mk_anon.
+
+  Definition wf_inputs (g : dcfg) : Prop :=
+    snd (ins g) = List.length (fst (ins g))
+    /\ List.incl (fst (ins g)) (inputs (graph g)).
+
+  Definition wf_outputs (g : dcfg) : Prop :=
+    snd (outs g) = List.length (fst (outs g))
+    /\ List.incl (fst (outs g)) (outputs (graph g)).
+
+  Definition wf_dcfg (g : dcfg) : Prop :=
+    wf_inputs g
+    /\ wf_outputs g.
+  
+  Definition empty_dcfg : dcfg := (mk_dcfg [] [] []).
+
+  Lemma empty_wf : wf_dcfg empty_dcfg.
+  Proof.
+    unfold empty_dcfg, wf_dcfg, wf_inputs, wf_outputs.
+    intuition.
+  Qed.
+
+  (* Could be a fresh/state monad *)
+  Record FST :=
+    mk_FST
+      {
+        counter_bid : nat ;
+        counter_reg : int ;
+        g : dcfg
+      }.
+
+  Definition fresh_init : FST :=
+    mk_FST 0 0%Z empty_dcfg.
+
+  Definition fresh : Type -> Type := fun X => FST -> (FST * X).
+  #[global] Instance freshM : Monad fresh :=
+    {|
+      ret := fun _ x s => (s,x);
+      bind := fun _ _ c k s => let '(s',x) := c s in k x s'
+    |}.
+
+  Definition freshLabel : fresh block_id :=
+    fun '(mk_FST bid reg g) => (mk_FST (S bid) reg g , name bid).
+
+  Definition freshReg : fresh int :=
+    fun '(mk_FST bid reg g) => (mk_FST bid (reg+1)%Z g, reg).
+
+  Definition setGraph g' : fresh unit :=
+    fun '(mk_FST bid reg g) => (mk_FST bid reg g', tt).
+
+End FreshnessMonad.
+
+Section InterfaceCombinators.
+
+  Notation code := (code typ).
+  Notation texp := (texp typ).
+
+  Definition mk_block (c : code) : fresh dcfg :=
+    input <- freshLabel ;;
+    output <- freshLabel ;;
+    let g := cfg_block c input output in
+    let dg := mk_dcfg g [input] [output] in
+    ret dg.
+
+  Definition mk_ret (c : code) (e : texp) : fresh dcfg :=
+    input <- freshLabel ;;
+    let g := cfg_ret c e input in
+    ret (mk_dcfg g [input] []).
+
+  Definition mk_seq (g1 g2 : dcfg) (out1 in2 : block_id) : fresh dcfg :=
+    let '(make_dcfg g1 (ins1, _) (outs1, _)) := g1 in
+    let '(make_dcfg g2 (ins2, _) (outs2, _)) := g2 in
+    let g := cfg_seq g1 g2 out1 in2 in
+    let ins := ins1++(remove in2 ins2) in
+    let outs := (remove out1 outs1)++outs2 in
+    let dg := mk_dcfg g ins outs in
+    ret dg.
+
+  Definition mk_join (g0: dcfg) (out1 out2 : block_id) : fresh dcfg :=
+    output <- freshLabel ;;
+    let '(make_dcfg g0 (ins0, _) (outs0, _)) := g0 in
+    let g := cfg_join g0 output out1 out2 in
+    let outs := (remove out1 outs0) in
+    let outs := (remove out2 outs) in
+    let outs := output::outs in
+    let dg := mk_dcfg g ins0 outs in
+    ret dg.
+
+  Definition mk_branch (cond : texp) (gT gF : dcfg)
+             (inT inF : block_id) : fresh dcfg :=
+    input <- freshLabel ;;
+    let '(make_dcfg gT (insT, _) (outsT, _)) := gT in
+    let '(make_dcfg gF (insF, _) (outsF, _)) := gF in
+    let g := cfg_branch cond gT gF input inT inF in
+    let ins := [input]
+                 ++ (remove inT insT)
+                 ++ (remove inF insF)
+    in
+    let outs := outsT++outsF in
+    let dg := mk_dcfg g ins outs in
+    ret dg.
+
+  Definition mk_while (expr_code : code) (cond : texp) (gBody : dcfg)
+             (inB outB : block_id) : fresh dcfg :=
+    input <- freshLabel ;;
+    output <- freshLabel ;;
+    let '(make_dcfg gBody (insBody, _) (outsBody, _)) := gBody in
+    let g := cfg_while_loop expr_code cond gBody input inB output outB in
+    let ins := [input] ++ (remove inB insBody) in
+    let outs := [output] ++ (remove outB outsBody) in
+    let dg := mk_dcfg g ins outs in
+    ret dg.
+
+End InterfaceCombinators.
+
+From Vellvm Require Import Utils.Tactics.
+
+Lemma wf_mk_block : forall σ c, wf_dcfg (snd ((mk_block c) σ )).
+Proof.
+  intros.
+  unfold wf_dcfg, wf_inputs, wf_outputs, mk_block.
+  destruct σ ; cbn.
+  unfold incl.
+  intuition
+  ; try reflexivity
+  ; try (cbn in * ; assumption).
+Qed.
+
+Lemma wf_mk_seq : forall σ g1 g2 out1 in2,
+    wf_dcfg g1 -> (* recursive use of the interface *)
+    wf_dcfg g2 ->
+    wf_dcfg (snd ((mk_seq g1 g2 out1 in2) σ )).
+Proof.
+  intros *  WF_G1 WF_G2.
+  unfold wf_dcfg, wf_inputs, wf_outputs, mk_seq.
+  destruct σ ; cbn.
+  unfold wf_dcfg, wf_inputs, wf_outputs in WF_G1, WF_G2.
+  destruct WF_G1 as [[LEN_INS_G1 INPUTS_G1] [LEN_OUT_G1 OUTPUTS_G1]].
+  destruct WF_G2 as [[LEN_INS_G2 INPUTS_G2] [LEN_OUT_G2 OUTPUTS_G2]].
+  unfold incl in *.
+  simpl in *.
+  intuition ;
+    repeat flatten_all.
+  - inv Heq0. reflexivity.
+  - unfold cfg_seq.
+    simpl in *.
+    rewrite Util.list_cons_app ;
+    rewrite !CFGC_Utils.inputs_app in *.
+    apply in_app_or in H.
+    apply in_or_app.
+    destruct H as [ H | H ].
+    + left. now apply INPUTS_G1.
+    + right ; apply in_or_app ; right.
+      apply INPUTS_G2.
+      rewrite remove_ListRemove in H ;
+      apply in_remove in H. intuition.
+  - inv Heq0. reflexivity.
+  - unfold cfg_seq.
+    simpl in *.
+    rewrite Util.list_cons_app ;
+    rewrite !ScopeTheory.outputs_app in *.
+    apply in_app_or in H.
+    apply in_or_app.
+    destruct H as [ H | H ].
+    + left. apply OUTPUTS_G1.
+      rewrite remove_ListRemove in H ;
+      apply in_remove in H. intuition.
+    + right ; apply in_or_app ; right.
+      now apply OUTPUTS_G2.
+Qed.
+
+Lemma wf_mk_join : forall σ g out1 out2,
+    wf_dcfg g ->
+    wf_dcfg (snd ((mk_join g out1 out2) σ)).
+Proof.
+  intros * WF_G.
+  unfold wf_dcfg, wf_inputs, wf_outputs, mk_seq.
+  destruct σ ; cbn.
+  unfold wf_dcfg, wf_inputs, wf_outputs in WF_G.
+  destruct WF_G as [[LEN_INS_G INPUTS_G] [LEN_OUT_G OUTPUTS_G]].
+  unfold incl in *.
+  repeat flatten_all.
+  simpl in *.
+  intuition.
+  - inv Heq0.
+    apply INPUTS_G in H.
+    unfold cfg_join.
+    rewrite Util.list_cons_app ;
+    rewrite !CFGC_Utils.inputs_app in *.
+    apply in_or_app. now left.
+  - rewrite H0.
+    unfold cfg_join.
+    rewrite Util.list_cons_app ;
+    rewrite !ScopeTheory.outputs_app in *.
+    apply in_or_app ; right. 
+    apply in_or_app ; right. simpl ; intuition.
+  - unfold cfg_join.
+    rewrite Util.list_cons_app
+    ; rewrite !ScopeTheory.outputs_app in *.
+    inv Heq1 ; clear H.
+    apply in_or_app ; left.
+    apply OUTPUTS_G.
+    rewrite remove_ListRemove in H0 ;
+      apply in_remove in H0 ; destruct H0 as [H0 _].
+    rewrite remove_ListRemove in H0 ;
+      apply in_remove in H0 ; destruct H0 as [H0 _].
+    assumption.
+Qed.
+    
+Lemma wf_mk_branch : forall σ cond gT gF inT inF,
+    wf_dcfg gT ->
+    wf_dcfg gF ->
+    wf_dcfg (snd ((mk_branch cond gT gF inT inF) σ)).
+Proof.
+  intros *  WF_GT WF_GF.
+  unfold wf_dcfg, wf_inputs, wf_outputs, mk_seq.
+  destruct σ ; cbn.
+  unfold wf_dcfg, wf_inputs, wf_outputs in WF_GT, WF_GF.
+  destruct WF_GT as [[LEN_INS_GT INPUTS_GT] [LEN_OUT_GT OUTPUTS_GT]].
+  destruct WF_GF as [[LEN_INS_GF INPUTS_GF] [LEN_OUT_GF OUTPUTS_GF]].
+  unfold incl in *.
+  simpl in *.
+  intuition ;
+    repeat flatten_all ; simpl in * ; try auto.
+  - intuition. right.
+    inv Heq0.
+    rewrite !ScopeTheory.inputs_app.
+    apply in_or_app.
+    apply in_app_or in H0.
+    destruct H0 ; [left ; apply INPUTS_GT | right ; apply INPUTS_GF] ;
+    now rewrite remove_ListRemove in H0
+    ; apply in_remove in H0
+    ; destruct H0 as [H0 _].
+  - inv Heq1. clear H0.
+    rewrite Util.list_cons_app
+    ; rewrite !ScopeTheory.outputs_app in *.
+    apply in_or_app ; right.
+    apply in_or_app.
+    apply in_app_or in H.
+    destruct H ; [left ; apply OUTPUTS_GT | right ; apply OUTPUTS_GF] ; assumption.
+Qed.
+
+Lemma wf_mk_while : forall σ expr_code cond gB inB outB,
+    wf_dcfg gB ->
+    wf_dcfg (snd ((mk_while expr_code cond gB inB outB) σ)).
+Proof.
+  intros * WF_G.
+  unfold wf_dcfg, wf_inputs, wf_outputs, mk_seq.
+  destruct σ ; cbn.
+  unfold wf_dcfg, wf_inputs, wf_outputs in WF_G.
+  destruct WF_G as [[LEN_INS_G INPUTS_G] [LEN_OUT_G OUTPUTS_G]].
+  unfold incl in *.
+  repeat flatten_all.
+  simpl in *.
+  intuition.
+  - inv Heq0.
+    right.
+    rewrite !ScopeTheory.inputs_app.
+    apply in_or_app ; left.
+    apply INPUTS_G.
+    now rewrite remove_ListRemove in H0
+    ; apply in_remove in H0.
+  - rewrite H0.
+    clear.
+    rewrite Util.list_cons_app
+    ; rewrite !ScopeTheory.outputs_app in *.
+    apply in_or_app ; left ; cbn ; intuition.
+  - inv Heq1.
+    rewrite Util.list_cons_app
+    ; rewrite !ScopeTheory.outputs_app in *.
+    apply in_or_app ; right.
+    apply in_or_app ; left.
+    apply OUTPUTS_G.
+    now rewrite remove_ListRemove in H0
+    ; apply in_remove in H0.
+Qed.
+
+
+From Coq Require Import Lia.
+Lemma neq_name : forall n1 n2, name n1 <> name n2 <-> n1 <> n2.
+Proof.
+  intros.
+  unfold name, mk_anon.
+  split ; intro.
+  - intros ->. now destruct H.
+  - apply inj_neq in H.
+    unfold Zne in H.
+    intro.
+    injection H0.
+    intro.
+    rewrite H1 in H .
+    contradiction.
+Qed.
+
+Lemma wf_mk_block_bind :
+  forall σ0 σ1 σ2 c1 c2 g1 g2,
+    (mk_block c1) σ0 = (σ1, g1) ->
+    (mk_block c2) σ1 = (σ2, g2) ->
+    independent_flows (graph g1) (graph g2).
+Proof.
+  intros.
+  unfold mk_block in *.
+  unfold freshLabel in *.
+  destruct σ0.
+  cbn in *.
+  inv H. inv H0.
+  simpl.
+  unfold independent_flows, no_duplicate_bid, no_reentrance.
+  unfold cfg_block.
+  cbn.
+  unfold Coqlib.list_disjoint.
+  intuition ; subst ;
+    repeat (
+        match goal with
+        | h:context[List.In _ [_]] |- _ => apply CFGC_Utils.In_singleton in h
+        end
+      )
+  ; rewrite H0 in H ; clear H0
+  ; match goal with
+    | h:context[ name ?x = name ?y ] |- _ =>
+        assert (contra : name x <> name y)
+        by (apply neq_name ; lia )
+    end ;
+    now apply contra in H.
+Qed.
